# Boss 目标圈

```
((x(C)-x(B)-y(C)+y(B)) (y-y(B)) + (-x(C) + x(B) -y(C) + y(B))(x-x(B)) <= 0 ∨ (-x(C)+x(B)-y(C)+y(B)) (y-y(B)) + (-x(C) + x(B) +y(C) - y(B)) (x-x(B)) <= 0) ∧ (0.88^2 ((x(C)-x(B))^2+(y(C)-y(B))^2) <= (x-x(B))^2+(y-y(B))^2 <= 0.9^2 ((x(C)-x(B))^2+(y(C)-y(B))^2) ∨ (0.95^2 ((x(C)-x(B))^2+(y(C)-y(B))^2) <= (x-x(B))^2+(y-y(B))^2 <= ((x(C)-x(B))^2+(y(C)-y(B))^2)) ∨ (((x(B)-x(C)) + √3 (y(B)-y(C))) (x + 0.2 x(B) - 1.2 x(C)) - (√3 (x(B)-x(C)) - (y(B)-y(C))) (y + 0.2 y(B) - 1.2 y(C)) >= 0 ∧ (-(x(B)-x(C)) + √3 (y(B)-y(C)))  (x + 0.2 x(B) - 1.2 x(C)) - (√3 (x(B)-x(C)) + (y(B)-y(C))) (y + 0.2 y(B) - 1.2 y(C)) <= 0 ∧ (x - 0.05 x(B) - 0.95 x(C)) (x(C) - x(B)) + (y - 0.05 y(B) - 0.95 y(C)) (y(C) - y(B)) >= 0))
```

# 单向扇形
```
((-sin(-θ/2) * (x(C) - x(B)) + cos(-θ/2) * (y(C) - y(B))) * (x - x(B)) - (cos(-θ/2) * (x(C) - x(B)) + sin(-θ/2) * (y(C) - y(B))) * (y - y(B)))((-sin(θ/2) * (x(C) - x(B)) + cos(θ/2) * (y(C) - y(B))) * (x - x(B)) - (cos(θ/2) * (x(C) - x(B)) + sin(θ/2) * (y(C) - y(B))) * (y - y(B))) <= 0
```

# 双向扇形

前后：

```
((-sin(-θ/2) * (x(C) - x(B)) + cos(-θ/2) * (y(C) - y(B))) * (x - x(B)) - (cos(-θ/2) * (x(C) - x(B)) + sin(-θ/2) * (y(C) - y(B))) * (y - y(B)))((-sin(θ/2) * (x(C) - x(B)) + cos(θ/2) * (y(C) - y(B))) * (x - x(B)) - (cos(θ/2) * (x(C) - x(B)) + sin(θ/2) * (y(C) - y(B))) * (y - y(B))) <= 0
```

左右：

```
((-cos(-θ/2) * (x(C) - x(B)) - sin(-θ/2) * (y(C) - y(B))) * (x - x(B)) - (-sin(-θ/2) * (x(C) - x(B)) + cos(-θ/2) * (y(C) - y(B))) * (y - y(B)))((-cos(θ/2) * (x(C) - x(B)) - sin(θ/2) * (y(C) - y(B))) * (x - x(B)) - (-sin(θ/2) * (x(C) - x(B)) + cos(θ/2) * (y(C) - y(B))) * (y - y(B))) <= 0
```

# 四向扇形

正：
```
((-sin(-θ/2) * (x(C) - x(B)) + cos(-θ/2) * (y(C) - y(B))) * (x - x(B)) - (cos(-θ/2) * (x(C) - x(B)) + sin(-θ/2) * (y(C) - y(B))) * (y - y(B)))((-sin(θ/2) * (x(C) - x(B)) + cos(θ/2) * (y(C) - y(B))) * (x - x(B)) - (cos(θ/2) * (x(C) - x(B)) + sin(θ/2) * (y(C) - y(B))) * (y - y(B))) <= 0 ∨ ((-cos(-θ/2) * (x(C) - x(B)) - sin(-θ/2) * (y(C) - y(B))) * (x - x(B)) - (-sin(-θ/2) * (x(C) - x(B)) + cos(-θ/2) * (y(C) - y(B))) * (y - y(B)))((-cos(θ/2) * (x(C) - x(B)) - sin(θ/2) * (y(C) - y(B))) * (x - x(B)) - (-sin(θ/2) * (x(C) - x(B)) + cos(θ/2) * (y(C) - y(B))) * (y - y(B))) <= 0
```
